Break ARMv8 instructions into sub-instructions

ARMv8.thy
@@ -6,14 +6,38 @@ chapter \<open>ARMv8\<close>
 
 section \<open>State Encoding\<close>
 
-type_synonym ('v,'r,'g) state = "(('g \<Rightarrow> 'v) \<times> ('r \<Rightarrow> 'v))"
-type_synonym ('v,'r,'g) pred = "('v,'r,'g) state \<Rightarrow> bool"
-type_synonym ('v,'r,'g) rpred = "('v,'r,'g) state \<Rightarrow> ('v,'r,'g) state \<Rightarrow> bool"
+type_synonym ('v,'r) state = "(('v \<Rightarrow> 'v) \<times> ('r \<Rightarrow> 'v))"
+type_synonym ('v,'r) pred = "('v,'r) state \<Rightarrow> bool"
+type_synonym ('v,'r) rpred = "('v,'r) state \<Rightarrow> ('v,'r) state \<Rightarrow> bool"
+
+named_theorems pred_defs
+definition conj  (infixr "\<and>\<^sub>p" 35)
+  where "conj l r \<equiv> \<lambda>m. (l m) \<and> (r m)"
+definition imp  (infixr "\<longrightarrow>\<^sub>p" 35)
+  where "imp l r \<equiv> \<lambda>m. (l m) \<longrightarrow> (r m)"
+definition entail (infix "\<turnstile>\<^sub>p" 25)
+  where "entail P Q \<equiv> \<forall>m. P m \<longrightarrow> Q m"
+definition assert
+  where "assert b \<equiv> \<lambda>m. b"
+declare assert_def [pred_defs]
+declare entail_def [pred_defs]
+declare conj_def [pred_defs]
+declare imp_def [pred_defs]
+definition stabilize 
+  where "stabilize R P \<equiv> \<lambda>m. \<forall>m'. R m m' \<longrightarrow> P m'"
+definition reflexive 
+  where "reflexive R \<equiv> \<forall>m . R m  m"
+definition transitive 
+  where "transitive R \<equiv> \<forall>m m' m''. R m m' \<longrightarrow> R m' m'' \<longrightarrow> R m m''"
+abbreviation PFalse 
+  where "PFalse \<equiv> \<lambda>m. False"
+abbreviation PTrue 
+  where "PTrue \<equiv> \<lambda>m. True"
 
 subsection \<open>Write Operations\<close>
 
-definition pair_upd1 :: "(('a \<Rightarrow> 'b) \<times> ('c \<Rightarrow> 'd)) \<Rightarrow> 'a \<Rightarrow> 'b \<Rightarrow> (('a \<Rightarrow> 'b) \<times> ('c \<Rightarrow> 'd))"
-  where "pair_upd1 f a b = (\<lambda>x. if x = a then b else (fst f) x, snd f)"
+definition pair_upd1 :: "(('v \<Rightarrow> 'v) \<times> ('c \<Rightarrow> 'v)) \<Rightarrow> 'c \<Rightarrow> 'v \<Rightarrow> (('v \<Rightarrow> 'v) \<times> ('c \<Rightarrow> 'v))"
+  where "pair_upd1 f a b = (\<lambda>x. if x = snd f a then b else (fst f) x, snd f)"
 
 definition pair_upd2 :: "(('a \<Rightarrow> 'b) \<times> ('c \<Rightarrow> 'd)) \<Rightarrow> 'c \<Rightarrow> 'd \<Rightarrow> (('a \<Rightarrow> 'b) \<times> ('c \<Rightarrow> 'd))"
   where "pair_upd2 f a b = (fst f, \<lambda>x. if x = a then b else (snd f) x)"
@@ -38,15 +62,16 @@ abbreviation rg
   where "rg r m \<equiv> (snd m) r"
 
 abbreviation ld
-  where "ld x m \<equiv> (fst m) x"
+  where "ld x m \<equiv> (fst m) (snd m x)"
 
 section \<open>Instruction Language Definition\<close>
 
 text \<open>Capture a simple set of instructions, covering memory operations and fences\<close>
 (* TODO: Need support for CAS and other RMW *)
-datatype ('v,'r,'g) inst =
-    Load 'r 'g
-  | Store 'g 'r
+datatype ('v,'r) inst =
+    Load1 'r 'v
+  | Load2 'r 'r 'v
+  | Store 'r 'r
   | Op 'r "'v \<Rightarrow> 'v \<Rightarrow> 'v" 'r 'r
   | Cond "'v \<Rightarrow> bool" 'r
   | Fence
@@ -58,84 +83,163 @@ abbreviation NCond
   where "NCond f r \<equiv> Cond (\<lambda>v. \<not> f v) r"
 
 text \<open>Instruction Behaviour\<close>
-fun beh\<^sub>i :: "('v,'r,'g) inst \<Rightarrow> ('v,'r,'g) state rel"
+fun beh\<^sub>i :: "('v,'r) inst \<Rightarrow> ('v,'r) state rel"
   where
     "beh\<^sub>i (Store x r) = {(m,m'). m' = m (x :=\<^sub>1 rg r m)}" |
-    "beh\<^sub>i (Load r y) = {(m,m'). m' = m (r :=\<^sub>2 ld y m)}" |
+    "beh\<^sub>i (Load1 y v) = {(m,m'). m' = m  \<and> v = ld y m}" |
+    "beh\<^sub>i (Load2 r y v) = {(m,m'). m' = m (r :=\<^sub>2 v)}" |
     "beh\<^sub>i (Op r\<^sub>t f r\<^sub>1 r\<^sub>2) = {(m,m'). m' = m (r\<^sub>t :=\<^sub>2 f (rg r\<^sub>1 m) (rg r\<^sub>2 m))}" |
     "beh\<^sub>i (Cond f r) = {(m,m'). m = m' \<and> f (rg r m)}" |
     "beh\<^sub>i _ = Id"
 
 subsection \<open>Reordering\<close>
 
+(*
 text \<open>Define forwarding as the elimination of loads given a store to the same address\<close>
-fun fwd :: "('v,'r,'g) inst \<Rightarrow> ('v,'r,'g) inst \<Rightarrow> ('v,'r,'g) inst" 
+fun fwd :: "('v,'r) inst \<Rightarrow> ('v,'r) inst \<Rightarrow> ('v,'r) inst" 
   ("_\<langle>_\<rangle>" [1000,0] 1000)
   where 
     "fwd (Load r\<^sub>2 y) (Store x r\<^sub>1) = (if (x = y) then Op r\<^sub>2 (\<lambda>x y. x) r\<^sub>1 r\<^sub>1 else Load r\<^sub>2 y)" |
-    "fwd \<alpha> _ = \<alpha>"
+    "fwd \<alpha> _ = \<alpha>" *)
 
-text \<open>Define reordering based on Colvin & Smith\<close>
-fun re :: "('v,'r,'g) inst \<Rightarrow> ('v,'r,'g) inst \<Rightarrow> bool" 
-  (infix "\<hookleftarrow>" 100)
+fun reads
+  where
+    "reads (Store x r) = {x,r}" |
+    "reads (Load1 y v) = {y}" |
+    "reads (Load2 r y v) = {r,y}" |
+    "reads (Op _ _ r\<^sub>1 r\<^sub>2) = {r\<^sub>1,r\<^sub>2}" |
+    "reads (Cond _ r) = {r}" |
+    "reads _ = {}"
+
+fun writes
+  where
+    "writes (Op r _ _ _) = {r}" |
+    "writes (Load2 r _ _) = {r}" |
+    "writes _ = {}"
+
+fun addrs
+  where
+    "addrs (Store x _) = {x}" |
+    "addrs (Load1 y _) = {y}" |
+    "addrs _ = {}"
+
+fun re :: "('v,'r) inst \<Rightarrow> ('v,'r) inst \<Rightarrow> bool" 
   where
     "re _ Fence = False" |
     "re Fence _ = False" |
     "re (Store _ _) StFence = False" |
     "re StFence (Store _ _) = False" | 
     "re (Cond _ _) CFence = False" |
-    "re CFence (Load _ _) = False" |
+    "re CFence (Load1 _ _) = False" |
+
     "re (Cond _ _) (Store _ _) = False" |
     "re (Cond _ r\<^sub>c) (Op r\<^sub>t _ r\<^sub>1 r\<^sub>2) = (r\<^sub>c \<noteq> r\<^sub>t)" |
-    "re (Cond _ r\<^sub>c) (Load r\<^sub>t _) = (r\<^sub>c \<noteq> r\<^sub>t)" |
-    "re (Store y r\<^sub>s) (Load r\<^sub>t x) = (r\<^sub>s \<noteq> r\<^sub>t \<and> x \<noteq> y)" |
-    "re (Store y _) (Store x _) = (x \<noteq> y)" |
-    "re (Store _ r\<^sub>s) (Op r\<^sub>t _ r\<^sub>1 r\<^sub>2) = (r\<^sub>s \<noteq> r\<^sub>t)" |
-    "re (Load r\<^sub>t y) (Load r\<^sub>t' x) = (r\<^sub>t \<noteq> r\<^sub>t' \<and> x \<noteq> y)" |
-    "re (Load r\<^sub>t y) (Store x r\<^sub>s) = (r\<^sub>s \<noteq> r\<^sub>t \<and> x \<noteq> y)" |
-    "re (Load r\<^sub>t _) (Op r\<^sub>t' _ r\<^sub>1 r\<^sub>2) = (r\<^sub>t \<noteq> r\<^sub>t' \<and> r\<^sub>t \<noteq> r\<^sub>1 \<and> r\<^sub>t \<noteq> r\<^sub>2)" |
-    "re (Load r\<^sub>t _) (Cond _ r\<^sub>s) = (r\<^sub>t \<noteq> r\<^sub>s)" |
-    "re (Op r\<^sub>t _ r\<^sub>1 r\<^sub>2) (Load r\<^sub>t' _) = (r\<^sub>t' \<noteq> r\<^sub>t \<and> r\<^sub>t' \<noteq> r\<^sub>1 \<and> r\<^sub>t' \<noteq> r\<^sub>2)" |
-    "re (Op r\<^sub>t _ r\<^sub>1 r\<^sub>2) (Store _ r\<^sub>s) = (r\<^sub>t \<noteq> r\<^sub>s)" |
+    "re (Cond _ r\<^sub>c) (Load2 r\<^sub>t _ _) = (r\<^sub>c \<noteq> r\<^sub>t)" |
+
+    "re (Store x r\<^sub>s) (Load2 r\<^sub>t _ _) = (r\<^sub>s \<noteq> r\<^sub>t \<and> x \<noteq> r\<^sub>t)" |
+    "re (Store x r\<^sub>s) (Op r\<^sub>t _ r\<^sub>1 r\<^sub>2) = (r\<^sub>s \<noteq> r\<^sub>t \<and> x \<noteq> r\<^sub>t)" |
+
+    "re (Load1 y _) (Load2 r\<^sub>t x _) = (y \<noteq> x \<and> r\<^sub>t \<noteq> y)" |
+    "re (Load1 y _) (Op r\<^sub>t _ r\<^sub>1 r\<^sub>2) = (y \<noteq> r\<^sub>t)" |
+
+    "re (Load2 r\<^sub>t x _) (Load1 y _) = (y \<noteq> x \<and> r\<^sub>t \<noteq> y)" |
+    "re (Load2 r\<^sub>t y _) (Load2 r\<^sub>t' x _) = (r\<^sub>t \<noteq> r\<^sub>t' \<and> r\<^sub>t \<noteq> x \<and> r\<^sub>t' \<noteq> y)" |
+    "re (Load2 r\<^sub>t _ _) (Store x r\<^sub>s) = (r\<^sub>s \<noteq> r\<^sub>t \<and> x \<noteq> r\<^sub>t)" |
+    "re (Load2 r\<^sub>t y _) (Op r\<^sub>t' _ r\<^sub>1 r\<^sub>2) = (r\<^sub>t \<noteq> r\<^sub>t' \<and> r\<^sub>t' \<noteq> y \<and> r\<^sub>t \<noteq> r\<^sub>1 \<and> r\<^sub>t \<noteq> r\<^sub>2)" |
+    "re (Load2 r\<^sub>t _ _) (Cond _ r\<^sub>s) = (r\<^sub>t \<noteq> r\<^sub>s)" |
+
+    "re (Op r\<^sub>t _ r\<^sub>1 r\<^sub>2) (Load1 y _) = (y \<noteq> r\<^sub>t)" |
+    "re (Op r\<^sub>t _ r\<^sub>1 r\<^sub>2) (Load2 r\<^sub>t' y _) = (r\<^sub>t' \<noteq> r\<^sub>t \<and> r\<^sub>t' \<noteq> r\<^sub>1 \<and> r\<^sub>t' \<noteq> r\<^sub>2 \<and> r\<^sub>t \<noteq> y)" |
+
+    "re (Op r\<^sub>t _ r\<^sub>1 r\<^sub>2) (Store x r\<^sub>s) = (r\<^sub>t \<noteq> r\<^sub>s \<and> r\<^sub>t \<noteq> x)" |
     "re (Op r\<^sub>t _ r\<^sub>1 r\<^sub>2) (Op r\<^sub>t' _ r\<^sub>1' r\<^sub>2') = (r\<^sub>t' \<noteq> r\<^sub>t \<and> r\<^sub>t' \<noteq> r\<^sub>1 \<and> r\<^sub>t' \<noteq> r\<^sub>2 \<and> r\<^sub>t \<noteq> r\<^sub>1' \<and> r\<^sub>t \<noteq> r\<^sub>2')" |
     "re (Op r\<^sub>t _ r\<^sub>1 r\<^sub>2) (Cond _ r\<^sub>s) = (r\<^sub>t \<noteq> r\<^sub>s)" |
+
     "re _ _ = True"
+
+lemma
+  "re \<alpha> \<beta> \<Longrightarrow> writes \<alpha> \<inter> writes \<beta> = {}"
+  by (cases \<alpha>; cases \<beta>; auto)
+
+lemma
+  "re \<alpha> \<beta> \<Longrightarrow> writes \<alpha> \<inter> reads \<beta> = {}"
+  by (cases \<alpha>; cases \<beta>; auto)
+
+lemma
+  "re \<alpha> \<beta> \<Longrightarrow> reads \<alpha> \<inter> writes \<beta> = {}"
+  by (cases \<alpha>; cases \<beta>; auto)
+
+
+
+text \<open>Define reordering based on Colvin & Smith\<close>
+fun re_m :: "('v,'r) inst \<Rightarrow> ('v,'r) inst \<Rightarrow> ('v,'r) pred" 
+  where
+    "re_m (Store y _) (Load1 x _) = (\<lambda>m. rg x m \<noteq> rg y m)" |
+    "re_m (Store y _) (Store x _) = (\<lambda>m. rg x m \<noteq> rg y m)" |
+    "re_m (Load1 y _) (Store x _) = (\<lambda>m. rg x m \<noteq> rg y m)" |
+    "re_m _ _ = PTrue"
 
 section \<open>Instruction Specification Language Definition\<close>
 
 text \<open>Wrap instructions in more abstract specification to facilitate verification\<close>
-type_synonym ('v,'r,'g) ispec = "(('v,'r,'g) pred\<times>('v,'r,'g) inst)"
+type_synonym ('v,'r) ispec = "(('v,'r) pred \<times> ('v,'r) pred \<times> ('v,'r) inst)"
 
 text \<open>Duplicate forwarding and reordering behaviour of underlying instruction\<close>
-(* TODO: We should provide a method to introduce new VCs for forwarded instructions *)
-fun fwd\<^sub>s :: "('v,'r,'g) ispec \<Rightarrow> ('v,'r,'g) ispec \<Rightarrow> ('v,'r,'g) ispec" 
-  where "fwd\<^sub>s (p,\<alpha>) (_,\<beta>) = (p,fwd \<alpha> \<beta>)" 
+fun fwd\<^sub>s :: "('v,'r) ispec \<Rightarrow> ('v,'r) ispec \<Rightarrow> ('v,'r) ispec" 
+  where 
+    "fwd\<^sub>s (vc,ts,\<alpha>) (_,_,\<beta>) = (if re \<beta> \<alpha> then (vc,ts \<and>\<^sub>p re_m \<beta> \<alpha>,\<alpha>) else (vc,PFalse,\<alpha>))" 
 
-fun re\<^sub>s :: "('v,'r,'g) ispec \<Rightarrow> ('v,'r,'g) ispec \<Rightarrow> bool" 
-  where "re\<^sub>s (_,\<alpha>) (_,\<beta>) = re \<alpha> \<beta>" 
+fun beh\<^sub>s :: "('v,'r) ispec \<Rightarrow> ('v,'r) state rel" 
+  where "beh\<^sub>s (_,ts,\<alpha>) = {(m,m'). (m,m') \<in> beh\<^sub>i \<alpha>}" 
 
-fun beh\<^sub>s :: "('v,'r,'g) ispec \<Rightarrow> ('v,'r,'g) state rel" 
-  where "beh\<^sub>s (p,\<alpha>) = beh\<^sub>i \<alpha>" 
+fun vc\<^sub>s :: "('v,'r) ispec \<Rightarrow> ('v,'r) state set" 
+  where "vc\<^sub>s (p,ts,\<alpha>) = {m. ts m \<longrightarrow> p m}" 
 
-fun vc\<^sub>s :: "('v,'r,'g) ispec \<Rightarrow> ('v,'r,'g) state set" 
-  where "vc\<^sub>s (p,\<alpha>) = Collect p" 
+(* does ts\<^sub>\<alpha> depend on writes in \<beta>? *)
+
+definition comp (infixr "\<otimes>" 60)
+  where "comp a b \<equiv> {((g,l),(g',l')). (\<exists>g'' l'' . ((g,l),(g'',l'')) \<in> a \<and> ((g'',l''),(g',l')) \<in> b)}"
+
+lemma
+  "re (snd (snd \<alpha>))  (snd (snd \<beta>)) \<Longrightarrow> beh\<^sub>s \<alpha> \<otimes> beh\<^sub>s \<beta> \<supseteq> {((g,l),(g',l')). (re_m (snd (snd \<alpha>))  (snd (snd \<beta>))) (g,l) \<and> g = g' \<and> l = l' } \<otimes> beh\<^sub>s (fwd\<^sub>s \<beta> \<alpha>) \<otimes> beh\<^sub>s \<alpha>"
+  apply (cases \<alpha>; cases \<beta>)
+  apply (case_tac c; case_tac ca)
+  by (auto simp: pred_defs pair_upd1_def pair_upd2_def comp_def split: if_splits)
+
+
+(*
+  apply (rename_tac vc\<^sub>\<alpha> ts\<^sub>\<alpha> a vc\<^sub>\<beta> ts\<^sub>\<beta> b x v r\<^sub>2 y v')
+  apply (auto simp: pred_defs comp_def pair_upd2_def)[1]
+  defer 1
+  apply (auto simp: pred_defs comp_def pair_upd1_def pair_upd2_def)[1]
+  defer 1
+  apply (auto simp: pred_defs comp_def pair_upd1_def pair_upd2_def)[1]
+  defer 1
+  apply (auto simp: pred_defs comp_def pair_upd1_def pair_upd2_def)[1]
+  apply (auto simp: pred_defs comp_def pair_upd1_def pair_upd2_def)[1]
+  apply (auto simp: pred_defs comp_def pair_upd1_def pair_upd2_def)[1]
+  apply (auto simp: pred_defs comp_def pair_upd1_def pair_upd2_def)[1]
+  apply (auto simp: pred_defs comp_def pair_upd1_def pair_upd2_def)[1]
+*)
+
+
 
 text \<open>Common case of a true verification condition\<close>
 abbreviation VC\<^sub>T
-  where "VC\<^sub>T \<alpha> \<equiv> (\<lambda>m. True,\<alpha>)"
+  where "VC\<^sub>T \<alpha> \<equiv> (PTrue,PTrue,\<alpha>)"
 
 section \<open>While Language Definition\<close>
 
-datatype ('v,'r,'g) lang =
+datatype ('v,'r) lang =
     Skip
-  | Inst "('v,'r,'g) ispec"
-  | Seq "('v,'r,'g) lang" "('v,'r,'g) lang"
-  | If "'v \<Rightarrow> bool" 'r "('v,'r,'g) lang" "('v,'r,'g) lang"
-  | While "'v \<Rightarrow> bool" 'r "('v,'r,'g) pred" "('v,'r,'g) lang"
+  | Inst "('v,'r) ispec"
+  | Seq "('v,'r) lang" "('v,'r) lang"
+  | If "'v \<Rightarrow> bool" 'r "('v,'r) lang" "('v,'r) lang"
+  | While "'v \<Rightarrow> bool" 'r "('v,'r) pred" "('v,'r) lang"
 
 text \<open>Convert the While language into the com language expected by the underlying logic\<close> 
 (* TODO: This should be later, closer to the soundness proof *)
-fun lift\<^sub>c :: "('v,'r,'g) lang \<Rightarrow> (('v,'r,'g) ispec,('v,'r,'g) state) com"
+fun lift\<^sub>c :: "('v,'r) lang \<Rightarrow> (('v,'r) ispec,('v,'r) state) com"
   where
     "lift\<^sub>c Skip = com.Nil" |
     "lift\<^sub>c (Inst \<alpha>) = Basic \<alpha>"|
