ARMv8_Rules.thy
@@ -1,87 +1,68 @@
 theory ARMv8_Rules
-  imports Refine ARMv8 
+  imports Refine ARMv82
 begin
-
-named_theorems pred_defs
-definition conj  (infixr "\<and>\<^sub>p" 35)
-  where "conj l r \<equiv> \<lambda>m. (l m) \<and> (r m)"
-definition entail (infix "\<turnstile>\<^sub>p" 25)
-  where "entail P Q \<equiv> \<forall>m. P m \<longrightarrow> Q m"
-definition assert
-  where "assert b \<equiv> \<lambda>m. b"
-declare assert_def [pred_defs]
-declare entail_def [pred_defs]
-declare conj_def [pred_defs]
-definition stabilize 
-  where "stabilize R P \<equiv> \<lambda>m. \<forall>m'. R m m' \<longrightarrow> P m'"
-definition reflexive 
-  where "reflexive R \<equiv> \<forall>m . R m  m"
-definition transitive 
-  where "transitive R \<equiv> \<forall>m m' m''. R m m' \<longrightarrow> R m' m'' \<longrightarrow> R m m''"
 
 section \<open>Predicate Transformations\<close>
 
+definition stabilize 
+  where "stabilize R P \<equiv> \<lambda>(g,l). \<forall>g'. R g g' \<longrightarrow> P (g',l)"
+
 text \<open>Transform a predicate based on an instruction\<close>
-fun wp\<^sub>i :: "('v,'r,'g) inst \<Rightarrow> ('v,'r,'g) pred \<Rightarrow> ('v,'r,'g) pred" 
+fun wp\<^sub>i :: "('v,'r) inst \<Rightarrow> ('v,'r) pred \<Rightarrow> ('v,'r) pred" 
   where 
-    "wp\<^sub>i (Store x r) Q = (\<lambda>m. Q (m (x :=\<^sub>1 rg r m)))" | 
-    "wp\<^sub>i (Load r x) Q = (\<lambda>m. Q (m (r :=\<^sub>2 ld x m)))" | 
-    "wp\<^sub>i (Op r\<^sub>t f r\<^sub>1 r\<^sub>2) Q = (\<lambda>m. Q (m (r\<^sub>t :=\<^sub>2 f (rg r\<^sub>1 m) (rg r\<^sub>2 m))))" |
-    "wp\<^sub>i (Cond f r) Q = (\<lambda>m. (f (rg r m)) \<longrightarrow> Q m)" | 
+    "wp\<^sub>i (load addr val) Q = (\<lambda>m. ld m addr = val \<longrightarrow> Q m)" | 
+    "wp\<^sub>i (store addr r) Q = (\<lambda>m. Q (m (addr :=\<^sub>1 rg m r)))" | 
+    "wp\<^sub>i (op r f rs) Q = (\<lambda>m. Q (m (r :=\<^sub>2 f (map (rg m) rs))))" |
+    "wp\<^sub>i (test f rs) Q = (\<lambda>m. f (map (rg m) rs) \<longrightarrow> Q m)" | 
     "wp\<^sub>i _ Q = Q"
 
-fun wp\<^sub>s  :: "('v,'r,'g) ispec \<Rightarrow> ('v,'r,'g) pred \<Rightarrow> ('v,'r,'g) pred"
-  where
-    "wp\<^sub>s (p,\<alpha>) Q = (p \<and>\<^sub>p wp\<^sub>i \<alpha> Q)"
-
 text \<open>The WP predicate transformer given a rely R and guarantee G\<close>
-fun wp :: "('v,'r,'g) rpred \<Rightarrow> ('v,'r,'g) rpred \<Rightarrow> ('v,'r,'g) lang \<Rightarrow> ('v,'r,'g) pred \<Rightarrow> ('v,'r,'g) pred"
+fun wp :: "('v,'r) rpred \<Rightarrow> ('v,'r) rpred \<Rightarrow> ('v,'r) lang \<Rightarrow> ('v,'r) pred \<Rightarrow> ('v,'r) pred"
   where
     "wp R G Skip Q = Q" |
-    "wp R G (Inst \<alpha>) Q = stabilize R (wp\<^sub>s \<alpha> Q)" |
+    "wp R G (Load vc r\<^sub>a r) Q = stabilize R (vc \<and>\<^sub>p (\<lambda>m. Q (m (r :=\<^sub>2 ld m (rg m r\<^sub>a)))))" |
+    "wp R G (Store vc r\<^sub>a r) Q = stabilize R (vc \<and>\<^sub>p (\<lambda>m. Q (m (rg m r\<^sub>a :=\<^sub>1 rg m r))))" |
+    "wp R G (Op r f rs) Q = wp\<^sub>i (op r f rs) Q" |
     "wp R G (Seq c\<^sub>1 c\<^sub>2) Q = wp R G c\<^sub>1 (wp R G c\<^sub>2 Q)" |
-    "wp R G (If f r c\<^sub>1 c\<^sub>2) Q = stabilize R (wp\<^sub>i (Cond f r) (wp R G c\<^sub>1 Q) \<and>\<^sub>p 
-                                           wp\<^sub>i (NCond f r) (wp R G c\<^sub>2 Q))" |
+    "wp R G (If f r c\<^sub>1 c\<^sub>2) Q = (wp\<^sub>i (test f r) (wp R G c\<^sub>1 Q) \<and>\<^sub>p wp\<^sub>i (ntest f r) (wp R G c\<^sub>2 Q))" |
     "wp R G (While f r I c) Q = (stabilize R I \<and>\<^sub>p
-                                (assert (I \<turnstile>\<^sub>p (wp\<^sub>i (Cond f r) (wp R G c (stabilize R I))) \<and>\<^sub>p 
-                                              wp\<^sub>i (NCond f r) Q)))"
+                                (assert (I \<turnstile>\<^sub>p (wp\<^sub>i (test f r) (wp R G c (stabilize R I))) \<and>\<^sub>p 
+                                              wp\<^sub>i (ntest f r) Q)))"
 
 text \<open>Convert a state predicate into the shallow-embedding\<close>
-definition state
-  where "state P \<equiv> {(m). P m}"
+abbreviation state
+  where "state P \<equiv> Collect P"
 
 text \<open>Convert a state relation into the shallow-embedding\<close>
-definition step
-  where "step P \<equiv> {((m),(m')). P m m'}"
+definition step\<^sub>R
+  where "step\<^sub>R P \<equiv> {((g,l),(g',l')). P g g' \<and> l = l'}"
+
+definition step\<^sub>G
+  where "step\<^sub>G P \<equiv> {((g,l),(g',l')). P g g'}"
 
 section \<open>Wellformedness\<close>
 
 text \<open>Couple all wellformedness conditions into a single definition\<close>
-definition wellformed :: "('v,'r,'g) rpred \<Rightarrow> ('v,'r,'g) rpred \<Rightarrow> ('v,'r,'g) pred \<Rightarrow> bool"
+definition wellformed :: "('v,'r) rpred \<Rightarrow> ('v,'r) rpred \<Rightarrow> ('v,'r) pred \<Rightarrow> bool"
   where "wellformed R G Q \<equiv> 
-    stable (step R) (state Q)  \<and> reflexive R \<and> transitive R \<and> reflexive G" 
-
-lemma G_refl [intro]:
-  assumes wf: "wellformed R G Q"
-  shows "G m m" 
-  using wf unfolding wellformed_def reflexive_def by blast
+    stable (step\<^sub>R R) (state Q) \<and> reflexive R \<and> transitive R \<and> reflexive G" 
 
 text \<open>Establish wellformedness of a false predicate\<close>
 lemma wf_false:
   "\<forall>m. \<not> P m \<Longrightarrow> wellformed R G Q \<Longrightarrow> wellformed R G P"
-  unfolding wellformed_def stable_def by (auto simp: state_def)
+  unfolding wellformed_def stable_def by (auto)
 
 text \<open>Show that a stabilized predicate is stable\<close>
 lemma stabilize_stable [intro]:
   assumes wf: "wellformed R G P"
-  shows "stable (step R) (state (stabilize R Q))"
-  unfolding stable_def state_def step_def
+  shows "stable (step\<^sub>R R) (state (stabilize R Q))"
+  unfolding stable_def step\<^sub>R_def
 proof (clarsimp)
-  fix m m'
-  assume a: "(stabilize R Q) m" "R m m'"
-  have "\<forall>m''. R m' m'' \<longrightarrow> R m m''"
+  fix g l g'
+  assume a: "(stabilize R Q) (g,l)" "R g g'"
+  have "\<forall>g''. R g' g'' \<longrightarrow> R g g''"
     using assms a(2) unfolding wellformed_def transitive_def by blast
-  thus "(stabilize R Q) m'" using a(1) by (auto simp: stabilize_def)
+  thus "(stabilize R Q) (g',l)" using a(1) by (auto simp: stabilize_def)
 qed
 
 text \<open>Stabilization preserves wellformedness\<close>
@@ -89,16 +70,10 @@ lemma stabilize_wellformed [intro]:
   assumes "wellformed R G P"
   shows "wellformed R G (stabilize R Q)" (is "wellformed R G ?P")
 proof -
-  have "stable (step R) (state ?P)" 
+  have "stable (step\<^sub>R R) (state ?P)" 
     using stabilize_stable assms by blast
   thus ?thesis using assms unfolding wellformed_def by blast
 qed
-
-text \<open>WP preserves wellformedness\<close>
-lemma wellformed_actI [intro]:
-  assumes "wellformed R G Q"
-  shows "wellformed R G (wp R G (Inst \<alpha>) Q)"
-  using assms wellformed_def by auto
 
 text \<open>Elimination rule to ignore the stabilization process\<close>
 lemma stabilizeE:
@@ -109,19 +84,21 @@ lemma stabilizeE:
 
 section \<open>Program Wellformedness\<close>
 
+(*
 text \<open>We require all instructions in a program to conform to the guarantee\<close>
 
 text \<open>Compute the verification condition necessary for an instruction to conform to a guarantee G\<close>
-definition guar\<^sub>i :: "('v,'r,'g) inst \<Rightarrow> ('v,'r,'g) rpred \<Rightarrow> ('v,'r,'g) pred"
-  where "guar\<^sub>i i G \<equiv> \<lambda>m. \<forall>m'. (m,m') \<in> beh\<^sub>i i \<longrightarrow> (G m m' \<or> m = m')"
+definition guar\<^sub>i :: "('v,'r) inst \<Rightarrow> ('v,'r) rpred \<Rightarrow> ('v,'r) pred"
+  where "guar\<^sub>i i G \<equiv> \<lambda>m. \<forall>m'. (m,m') \<in> beh\<^sub>i i \<longrightarrow> (G (fst m) (fst m') \<or> m = m')"
 
-fun guar\<^sub>s :: "('v,'r,'g) ispec \<Rightarrow> ('v,'r,'g) rpred \<Rightarrow> bool"
-  where "guar\<^sub>s (p,\<alpha>) G = (p \<turnstile>\<^sub>p guar\<^sub>i \<alpha> G)"
+fun guar\<^sub>s :: "('v,'r) ispec \<Rightarrow> ('v,'r) rpred \<Rightarrow> bool"
+  where "guar\<^sub>s (p,ts,\<alpha>) G = (p \<and>\<^sub>p ts \<turnstile>\<^sub>p guar\<^sub>i \<alpha> G)"
+*)
 
 text \<open>Ensure all operations have preconditions strong enough to discharge their guarantee\<close>
 fun guar\<^sub>c
   where
-    "guar\<^sub>c (Inst \<alpha>) G = guar\<^sub>s \<alpha> G" |
+    "guar\<^sub>c (Store vc r\<^sub>a r) G = (\<forall>m. vc m \<longrightarrow> G (fst m) ((fst m)(rg m r\<^sub>a := rg m r)))" |
     "guar\<^sub>c (Seq c\<^sub>1 c\<^sub>2) G = (guar\<^sub>c c\<^sub>1 G \<and> guar\<^sub>c c\<^sub>2 G)" |
     "guar\<^sub>c (If f v c\<^sub>1 c\<^sub>2) G = (guar\<^sub>c c\<^sub>1 G \<and> guar\<^sub>c c\<^sub>2 G)" |
     "guar\<^sub>c (While f v I c) G = (guar\<^sub>c c G)" |
@@ -129,10 +106,26 @@ fun guar\<^sub>c
 
 section \<open>Soundness\<close>
 
+text \<open>Convert the While language into the com language expected by the underlying logic\<close> 
+fun lift\<^sub>c :: "('v,'r) lang \<Rightarrow> (('v,'r) ispec,('v,'r) state) com"
+  where
+    "lift\<^sub>c Skip = com.Nil" |
+    "lift\<^sub>c (Load vc r\<^sub>a r) = \<Sqinter> {[\<lfloor>eq r\<^sub>a v\<^sub>a\<rfloor>, \<lfloor>(\<lambda>m. rg m r\<^sub>a = v\<^sub>a) \<and>\<^sub>p vc,load v\<^sub>a v\<rfloor>, \<lfloor>assign r v\<rfloor>] |v v\<^sub>a. True}" |
+    "lift\<^sub>c (Store vc r\<^sub>a r) = \<Sqinter> {[\<lfloor>eq r\<^sub>a v\<^sub>a\<rfloor>, \<lfloor>(\<lambda>m. rg m r\<^sub>a = v\<^sub>a) \<and>\<^sub>p vc,store v\<^sub>a r\<rfloor>] |v\<^sub>a. True}" |
+    "lift\<^sub>c (Op r f rs) = Basic (\<lfloor>op r f rs\<rfloor>)" |
+    "lift\<^sub>c (Seq c\<^sub>1 c\<^sub>2) = (lift\<^sub>c c\<^sub>1 ; lift\<^sub>c c\<^sub>2)" |
+    "lift\<^sub>c (If f r c\<^sub>1 c\<^sub>2) = (Choice (com.Seq (Basic (\<lfloor>test f r\<rfloor>)) (lift\<^sub>c c\<^sub>1)) 
+                                    (com.Seq (Basic (\<lfloor>ntest f r\<rfloor>)) (lift\<^sub>c c\<^sub>2)))" |
+    "lift\<^sub>c (While f r I c) = (com.Seq ((com.Seq (Basic (\<lfloor>test f r\<rfloor>)) (lift\<^sub>c c))*) 
+                                      (Basic (\<lfloor>ntest f r\<rfloor>)))"
+
 subsection \<open>Interpretation of General Logic\<close>
 
-fun act_ref :: "('v,'r,'g) ispec \<Rightarrow> ('v,'r,'g) ispec \<Rightarrow> bool" 
+fun act_ref :: "('v,'r) ispec \<Rightarrow> ('v,'r) ispec \<Rightarrow> bool" 
   where "act_ref (p,\<alpha>) (q,\<beta>) = (\<alpha> = \<beta> \<and> (p \<turnstile>\<^sub>p q))"
+
+fun re\<^sub>s :: "('v,'r) ispec \<Rightarrow> ('v,'r) ispec \<Rightarrow> bool" 
+  where "re\<^sub>s (_,\<alpha>) (_,\<beta>) = re\<^sub>i \<alpha> \<beta>" 
 
 interpretation refine vc\<^sub>s beh\<^sub>s fwd\<^sub>s re\<^sub>s act_ref
   by (unfold_locales) (auto simp: pred_defs)
@@ -144,10 +137,10 @@ abbreviation rules_abv ("_,_ \<turnstile> _ {_} _" [20,0,0,0,20] 20)
   where "rules_abv \<equiv> rules"
 
 abbreviation lifted_abv ("_,_ \<turnstile>\<^sub>s _ {_} _" [20,0,0,0,20] 20)
-  where "lifted_abv R G P c Q \<equiv> step R,step G \<turnstile>\<^sub>l state P {lift\<^sub>c c} state Q"
+  where "lifted_abv R G P c Q \<equiv> step\<^sub>R R,step\<^sub>G G \<turnstile>\<^sub>l state P {lift\<^sub>c c} state Q"
 
 abbreviation validity_abv  ("\<Turnstile> _ SAT [_, _, _, _]" [60,0,0,0,0] 45) 
-  where "validity_abv c P R G Q \<equiv> validity (lift\<^sub>c c) (state P) (step R) (step G) (state Q)"
+  where "validity_abv c P R G Q \<equiv> validity (lift\<^sub>c c) (state P) (step\<^sub>R R) (step\<^sub>G G) (state Q)"
 
 text \<open>An ordering property on contexts\<close>
 definition context_order 
@@ -161,6 +154,110 @@ definition valid
 
 subsection \<open>Instruction Soundness\<close>
 
+lemma load_sound:
+  assumes "wellformed R G Q"
+  shows "R,G \<turnstile>\<^sub>s wp R G (Load vc r\<^sub>a r) Q {Load vc r\<^sub>a r} Q"
+proof (clarsimp, rule lrules.bigchoice, clarsimp, intro lrules.ord lrules.basic)
+  show "step\<^sub>R R,step\<^sub>G G \<turnstile>\<^sub>l state Q {com.Nil} state Q"
+    using assms by (auto simp: wellformed_def)
+next
+  fix v
+  show "atomic_rule (step\<^sub>R R) (step\<^sub>G G) (state (wp\<^sub>i (assign r v) Q)) (\<lfloor>assign r v\<rfloor>) (state Q)"
+    unfolding atomic_rule_def
+    apply (intro conjI)    apply (clarsimp simp add: wp_def)
+    using assms 
+    apply (clarsimp simp add: step\<^sub>G_def pair_upd2_def wellformed_def reflexive_def)
+    using assms
+    apply (clarsimp simp add: step\<^sub>G_def pair_upd2_def wellformed_def stable_def step\<^sub>R_def)
+    apply (metis (full_types) snd_conv)
+    using assms
+    apply (clarsimp simp add: step\<^sub>G_def pair_upd2_def wellformed_def stable_def step\<^sub>R_def)
+    done
+next
+  fix v v\<^sub>a
+  show "atomic_rule (step\<^sub>R R) (step\<^sub>G G) 
+        (state (stabilize R ((\<lambda>m. rg m r\<^sub>a = v\<^sub>a) \<and>\<^sub>p vc \<and>\<^sub>p wp\<^sub>i (load v\<^sub>a v) (wp\<^sub>i (assign r v) Q))))
+        (\<lfloor>(\<lambda>m. rg m r\<^sub>a = v\<^sub>a) \<and>\<^sub>p vc,load v\<^sub>a v\<rfloor>) 
+        (state (wp\<^sub>i (assign r v) Q))"
+    unfolding atomic_rule_def
+    apply (intro conjI)
+    using assms
+    apply (auto simp: wp_def pred_defs elim!: stabilizeE)
+    apply (clarsimp simp add: step\<^sub>G_def pair_upd2_def wellformed_def stable_def step\<^sub>R_def)
+    apply (metis (full_types) snd_conv)
+    done
+next
+  fix v v\<^sub>a
+  show "atomic_rule (step\<^sub>R R) (step\<^sub>G G)
+        (state
+          (ARMv8_Rules.stabilize R
+            (vc \<and>\<^sub>p (\<lambda>m. Q (m(r :=\<^sub>2 ld m (rg m r\<^sub>a)))))))
+        (\<lfloor>eq r\<^sub>a v\<^sub>a\<rfloor>)
+        (state
+          (ARMv8_Rules.stabilize R
+            ((\<lambda>m. rg m r\<^sub>a = v\<^sub>a) \<and>\<^sub>p vc \<and>\<^sub>p wp\<^sub>i (load v\<^sub>a v) (wp\<^sub>i (assign r v) Q))))"
+    unfolding atomic_rule_def
+    apply (intro conjI)
+    using assms
+    apply (auto simp: wp_def pred_defs)
+    by (auto simp: stabilize_def)
+qed
+
+lemma store_sound:
+  assumes "wellformed R G Q" "guar\<^sub>c (Store vc r\<^sub>a r) G"
+  shows "R,G \<turnstile>\<^sub>s wp R G (Store vc r\<^sub>a r) Q {Store vc r\<^sub>a r} Q"
+proof (clarsimp, rule lrules.bigchoice, clarsimp, intro lrules.ord lrules.basic)
+  show "step\<^sub>R R,step\<^sub>G G \<turnstile>\<^sub>l state Q {com.Nil} state Q"
+    using assms by (auto simp: wellformed_def)
+next
+  fix v v\<^sub>a
+  show "atomic_rule (step\<^sub>R R) (step\<^sub>G G) 
+          (state (stabilize R (((\<lambda>m. rg m r\<^sub>a = v\<^sub>a \<and> rg m r = v) \<and>\<^sub>p vc) \<and>\<^sub>p wp\<^sub>i (store v\<^sub>a v) Q)))
+          (\<lfloor>(\<lambda>m. rg m r\<^sub>a = v\<^sub>a \<and> rg m r = v) \<and>\<^sub>p vc,store v\<^sub>a v\<rfloor>) 
+          (state Q)"
+    unfolding atomic_rule_def
+    apply (intro conjI)    
+    using assms
+    apply (auto simp: wp_def pred_defs step\<^sub>G_def pair_upd1_def elim!: stabilizeE split: if_splits)
+    apply (subgoal_tac "(a(b r\<^sub>a := b r)) = (\<lambda>x. if x = b r\<^sub>a then rg (\<lfloor>a,b\<rfloor>) r else ld (\<lfloor>a,b\<rfloor>) x)")
+    apply metis
+    apply auto[1]
+    by (auto simp: wellformed_def)
+next
+  fix v v\<^sub>a
+  show "atomic_rule (step\<^sub>R R) (step\<^sub>G G) 
+        (state (ARMv8_Rules.stabilize R (((\<lambda>m. rg m r\<^sub>a = v\<^sub>a) \<longrightarrow>\<^sub>p ((\<lambda>m. rg m r = v) \<and>\<^sub>p vc) \<and>\<^sub>p wp\<^sub>i (store v\<^sub>a v) Q))))
+        (\<lfloor>eq r\<^sub>a v\<^sub>a\<rfloor>)
+        (state (ARMv8_Rules.stabilize R (((\<lambda>m. rg m r\<^sub>a = v\<^sub>a \<and> rg m r = v) \<and>\<^sub>p vc) \<and>\<^sub>p wp\<^sub>i (store v\<^sub>a v) Q)))"
+    unfolding atomic_rule_def
+    apply (intro conjI)
+    using assms
+    apply (auto simp: wp_def pred_defs)
+    by (auto simp: stabilize_def)
+next
+  fix v v\<^sub>a
+  show "atomic_rule (step\<^sub>R R) (step\<^sub>G G)
+        (state (ARMv8_Rules.stabilize R (vc \<and>\<^sub>p (\<lambda>m. Q (m(rg m r\<^sub>a :=\<^sub>1 rg m r))))))
+        (\<lfloor>eq r v\<rfloor>)
+        (state (ARMv8_Rules.stabilize R ((\<lambda>m. rg m r\<^sub>a = v\<^sub>a) \<longrightarrow>\<^sub>p ((\<lambda>m. rg m r = v) \<and>\<^sub>p vc) \<and>\<^sub>p wp\<^sub>i (store v\<^sub>a v) Q)))"
+    unfolding atomic_rule_def
+    apply (intro conjI)
+    using assms
+    apply (auto simp: wp_def pred_defs)
+    by (auto simp: stabilize_def)
+qed    
+
+lemma op_sound:
+  assumes "wellformed R G Q"
+  shows "R,G \<turnstile>\<^sub>s wp R G (Op r f rs) Q {Op r f rs} Q"
+  apply (clarsimp, rule lrules.basic, simp add: atomic_rule_def, intro conjI)
+  using assms
+  apply (auto simp: wp_def pred_defs step\<^sub>G_def pair_upd2_def wellformed_def reflexive_def)
+  apply (auto simp: stable_def step\<^sub>R_def)
+  by (metis snd_conv)
+
+
+(*
 text \<open>WP correctly transforms the state for an instruction\<close>
 lemma wp_sound [intro]:
   assumes wf: "wellformed R G Q" 
@@ -192,6 +289,7 @@ proof (rule lrules.conseq)
   show "state P \<subseteq> state (wp R G (Inst \<alpha>) Q)"
     using assms(3) by (auto simp: entail_def state_def)
 qed auto
+*)
 
 subsection \<open>Base Introduction Rules\<close>
 
@@ -217,23 +315,31 @@ lemma skipWP:
   "R,G \<turnstile>\<^sub>w Q {Skip} Q"
   by (auto simp: context_order_def valid_def wellformed_def)
 
+(*
 text \<open>Instruction Rule\<close>
 lemma instWP:
   "R,G \<turnstile>\<^sub>w wp R G (Inst \<alpha>) Q {Inst \<alpha>} Q"
   unfolding valid_def using inst_sound[of R G Q \<alpha>] by auto
- 
+ *)
+
 text \<open>Sequential Rule\<close>
 lemma seqWP:
   "R,G \<turnstile>\<^sub>w P {c\<^sub>1} Q \<Longrightarrow> R,G \<turnstile>\<^sub>w M {c\<^sub>2} P \<Longrightarrow> R,G \<turnstile>\<^sub>w M {Seq c\<^sub>2 c\<^sub>1} Q"
   unfolding valid_def by auto
 
+(*
 lemma guar_cond [simp]:
   "guar\<^sub>i (Cond f r) G = (\<lambda>m. True)"
   by (auto simp add: pred_defs guar\<^sub>i_def)
+*)
 
 lemma [simp]:
   "(P \<turnstile>\<^sub>p P) = True"
-  by (auto simp add: pred_defs guar\<^sub>i_def)
+  by (auto simp add: pred_defs)
+
+lemma [simp]:
+  "(PTrue \<and>\<^sub>p PTrue) = PTrue"
+  by (auto simp: pred_defs)
 
 text \<open>Stabilization preserves entailment\<close>
 lemma stabilize_entail [intro]:
@@ -241,35 +347,61 @@ lemma stabilize_entail [intro]:
   shows "stabilize R P \<turnstile>\<^sub>p stabilize R Q"
   using assms by (clarsimp simp add: entail_def stabilize_def)
 
+lemma stabilize_entail' [intro]:
+  assumes "wellformed R G Z"
+  assumes "P \<turnstile>\<^sub>p Q"
+  shows "stabilize R P \<turnstile>\<^sub>p Q"
+  using assms
+  by (clarsimp simp add: entail_def stabilize_def wellformed_def stable_def step\<^sub>R_def reflexive_def)
+
+lemma test_sound:
+  assumes "wellformed R G Q"
+  assumes "P \<turnstile>\<^sub>p wp\<^sub>i (test f rs) Q"
+  shows "step\<^sub>R R,step\<^sub>G G \<turnstile>\<^sub>l state P {Basic (\<lfloor>test f rs\<rfloor>)} state Q"
+  apply (rule lrules.conseq[of "step\<^sub>R R" "step\<^sub>G G" "state (wp\<^sub>i (test f rs) Q)" _ "state Q"])
+  apply (rule lrules.basic)
+  unfolding atomic_rule_def
+  apply (intro conjI)
+  apply (clarsimp simp: wp_def)
+  apply (clarsimp)
+  using assms apply (auto simp: wellformed_def step\<^sub>R_def stable_def)[2]
+  using assms(2) apply (clarsimp simp: pred_defs)[1]
+  by auto
+
 text \<open>If Rule\<close>
 lemma ifWP:
   assumes "R,G \<turnstile>\<^sub>w P\<^sub>1 {c\<^sub>1} Q"
   assumes "R,G \<turnstile>\<^sub>w P\<^sub>2 {c\<^sub>2} Q"
-  shows "R,G \<turnstile>\<^sub>w stabilize R (wp\<^sub>i (Cond f r) P\<^sub>1 \<and>\<^sub>p wp\<^sub>i (NCond f r) P\<^sub>2) {If f r c\<^sub>1 c\<^sub>2} Q"
-  using assms 
+  shows "R,G \<turnstile>\<^sub>w (wp\<^sub>i (test f r) P\<^sub>1 \<and>\<^sub>p wp\<^sub>i (ntest f r) P\<^sub>2) {If f r c\<^sub>1 c\<^sub>2} Q"
+  using assms
   apply (clarsimp simp add: valid_def)
   apply (intro impI conjI lrules.choice lrules.seq stabilize_wellformed; assumption?)
-  by (intro inst_conseq; simp; intro stabilize_entail; simp add: pred_defs)+
+  apply (rule test_sound; simp)
+  apply (simp add: pred_defs)
+  apply (rule test_sound; simp)
+  apply (simp add: pred_defs)
+  unfolding wellformed_def
+  apply simp
+  by (auto simp: stable_def step\<^sub>R_def pred_defs)
 
 text \<open>While Rule\<close>
 lemma whileWP:
-  assumes "I \<turnstile>\<^sub>p wp\<^sub>i (Cond f r) P \<and>\<^sub>p wp\<^sub>i (NCond f r) Q"
+  assumes "I \<turnstile>\<^sub>p wp\<^sub>i (test f r) P \<and>\<^sub>p wp\<^sub>i (ntest f r) Q"
   assumes "R,G \<turnstile>\<^sub>w P {c} stabilize R I" (is "R,G \<turnstile>\<^sub>w P {c} ?I")
   shows "R,G \<turnstile>\<^sub>w ?I {While f r I c} Q"
   unfolding valid_def lift\<^sub>c.simps
 proof (intro impI conjI lrules.choice lrules.seq stabilize_wellformed; assumption?)
   assume "guar\<^sub>c (While f r I c) G \<and> wellformed R G Q"
-  thus "step R,step G \<turnstile>\<^sub>l (state ?I) {Basic (VC\<^sub>T (NCond f r))} state Q"
-    using assms(1) 
-    by (intro inst_conseq; simp; intro stabilize_entail; simp add: pred_defs)
+  thus "step\<^sub>R R,step\<^sub>G G \<turnstile>\<^sub>l (state ?I) {Basic (\<lfloor>ntest f r\<rfloor>)} state Q"
+    using assms(1) by (intro test_sound; simp; intro stabilize_entail'; simp add: pred_defs)
 next
   assume "guar\<^sub>c (While f r I c) G \<and> wellformed R G Q"
   hence "guar\<^sub>c c G" "wellformed R G ?I" by auto
-  thus "step R,step G \<turnstile>\<^sub>l state ?I {(Basic (VC\<^sub>T (Cond f r)) ; lift\<^sub>c c)*} state ?I"
+  thus "step\<^sub>R R,step\<^sub>G G \<turnstile>\<^sub>l state ?I {(Basic (\<lfloor>test f r\<rfloor>) ; lift\<^sub>c c)*} state ?I"
     using assms
     apply (intro lrules.loop lrules.seq stabilize_stable; simp add: valid_def)
     defer 1
-    by blast (intro inst_conseq; simp; intro stabilize_entail; simp add: pred_defs)
+    by blast (intro test_sound; simp; intro stabilize_entail'; simp add: pred_defs)
 qed auto
 
 lemma local_lift [intro]:
@@ -277,16 +409,22 @@ lemma local_lift [intro]:
   by (induct c) auto
 
 lemma guar_all:
-  "guar\<^sub>c c G \<Longrightarrow> \<forall>\<beta>\<in>basics (lift\<^sub>c c). guar \<beta> (step G)"
-  by (induct c) auto
+  "wellformed R G Q \<Longrightarrow> guar\<^sub>c c G \<Longrightarrow> \<forall>\<beta>\<in>basics (lift\<^sub>c c). guar \<beta> (step\<^sub>G G)"
+  apply (induct c) 
+  apply (auto simp: step\<^sub>G_def pair_upd1_def pair_upd2_def pred_defs wellformed_def reflexive_def)
+  apply (subgoal_tac "G aa (aa(ba x2 := ba x3))")
+  apply (subgoal_tac "(aa(ba x2 := ba x3)) = (\<lambda>x. if x = ba x2 then ba x3 else ld (\<lfloor>aa,ba\<rfloor>) x)")
+  apply simp
+  apply auto
+  done
 
 text \<open>False Rule\<close>
 lemma falseWP:
   assumes "P \<turnstile>\<^sub>p (\<lambda>m. False)"
   shows "R,G \<turnstile>\<^sub>w P {c} Q"
   using assms unfolding valid_def
-  apply (intro conjI impI guar_all lrules.conseq[OF falseI, where ?G="step G"])
-  by (auto simp: entail_def state_def intro: wf_false)
+  apply (intro conjI impI guar_all lrules.conseq[OF falseI, where ?G="step\<^sub>G G"])
+  by (auto simp: entail_def intro: wf_false)
 
 text \<open>Precondition Rewrite Rule\<close>
 lemma rewriteWP:
@@ -294,7 +432,7 @@ lemma rewriteWP:
 proof (clarsimp simp add: valid_def context_order_def)
   assume a: "M \<turnstile>\<^sub>p P"
   assume "R,G \<turnstile>\<^sub>s P {c} Q "
-  thus "R,G \<turnstile>\<^sub>s M {c} Q" by (rule lrules.conseq) (insert a, auto simp: entail_def state_def)
+  thus "R,G \<turnstile>\<^sub>s M {c} Q" by (rule lrules.conseq) (insert a, auto simp: entail_def)
 qed
 
 text \<open>Assert Rule\<close>
@@ -318,15 +456,17 @@ lemma skipRW:
   shows "R,G \<turnstile>\<^sub>w P {Skip} Q"
   using rewriteWP[OF skipWP assms] .
 
+(*
 text \<open>Act Rewrite Rule\<close>
 lemma actRW:
   assumes "R,G \<turnstile>\<^sub>w P \<ge> wp R G (Inst \<alpha>) Q"
   shows "R,G \<turnstile>\<^sub>w P {Inst \<alpha>} Q"
   using rewriteWP[OF instWP assms] .
+*)
 
 text \<open>If Rewrite Rule\<close>
 lemma ifRW:
-  assumes "R,G \<turnstile>\<^sub>w P \<ge> stabilize R (wp\<^sub>i (Cond f r) P\<^sub>1 \<and>\<^sub>p wp\<^sub>i (NCond f r) P\<^sub>2)"
+  assumes "R,G \<turnstile>\<^sub>w P \<ge> (wp\<^sub>i (test f r) P\<^sub>1 \<and>\<^sub>p wp\<^sub>i (ntest f r) P\<^sub>2)"
   assumes "R,G \<turnstile>\<^sub>w P\<^sub>1 {c\<^sub>1} Q"
   assumes "R,G \<turnstile>\<^sub>w P\<^sub>2 {c\<^sub>2} Q"
   shows "R,G \<turnstile>\<^sub>w P {If f r c\<^sub>1 c\<^sub>2} Q"
@@ -336,11 +476,18 @@ text \<open>While Rewrite Rule\<close>
 lemma whileRW:
   assumes order: "R,G \<turnstile>\<^sub>w N \<ge> stabilize R I"
   assumes recur: "R,G \<turnstile>\<^sub>w P {c} stabilize R I"
-  assumes side: "I \<turnstile>\<^sub>p wp\<^sub>i (Cond f r) P \<and>\<^sub>p wp\<^sub>i (NCond f r) Q"
+  assumes side: "I \<turnstile>\<^sub>p wp\<^sub>i (test f r) P \<and>\<^sub>p wp\<^sub>i (ntest f r) Q"
   shows "R,G \<turnstile>\<^sub>w N {While f r I c} Q"
   using rewriteWP[OF whileWP[OF side recur] order] .
 
 subsection \<open>Soundness\<close>
+
+lemma wellformed_op:
+  assumes "wellformed R G Q"
+  shows "wellformed R G (ARMv8_Rules.wp R G (Op x1 x2 x3) Q)"
+  using assms unfolding wellformed_def
+  apply (auto simp: stable_def step\<^sub>R_def pair_upd2_def)
+  by (metis snd_conv) 
 
 lemma wp_valid:
   shows "R,G \<turnstile>\<^sub>w wp R G c Q {c} Q" 
@@ -348,14 +495,20 @@ proof (induct c arbitrary: Q)
   case Skip
   thus ?case using skipWP by auto
 next
-  case (Inst \<beta>)
-  thus ?case using instWP by blast
+  case (Load)
+  thus ?case using load_sound by (auto simp: valid_def) 
+next
+  case (Store)
+  thus ?case using store_sound by (auto simp: valid_def) 
+next
+  case (Op)
+  thus ?case using op_sound wellformed_op unfolding valid_def by metis
 next
   case (Seq c\<^sub>1 c\<^sub>2)
   thus ?case using seqWP unfolding wp.simps by blast
 next
   case (If f r c\<^sub>1 c\<^sub>2)
-  thus ?case using ifWP unfolding wp.simps by metis
+  thus ?case using ifWP unfolding wp.simps by blast
 next
   case (While f r I c)
   thus ?case unfolding wp.simps
@@ -365,18 +518,19 @@ qed
 text \<open>Soundness lemma for WP reasoning over ARMv8 with verification conditions\<close>
 theorem armv8_wp_sound_vc:
   assumes wf: "transitive R" "reflexive R" "reflexive G" 
-  assumes st: "stable (step R) (state Q)" 
+  assumes st: "stable (step\<^sub>R R) (state Q)" 
   assumes g: "guar\<^sub>c c G"
   assumes P: "P \<turnstile>\<^sub>p wp R G c Q"
-  assumes i: "inter (step R) (step G) (lift\<^sub>c c)" (* Rephrase this in terms of the ARMv8 analysis *)
+  assumes i: "inter (step\<^sub>R R) (step\<^sub>G G) (lift\<^sub>c c)" (* Rephrase this in terms of the ARMv8 analysis *)
   shows "\<Turnstile> c SAT [P, R, G, Q]"
 proof -
   have "wellformed R G Q" using wf st by (auto simp: wellformed_def)
   hence "R,G \<turnstile>\<^sub>s wp R G c Q {c} Q" using g wp_valid unfolding valid_def by blast
-  hence "R,G \<turnstile>\<^sub>s P {c} Q" by (rule lrules.conseq) (insert P, auto simp: state_def entail_def)
+  hence "R,G \<turnstile>\<^sub>s P {c} Q" by (rule lrules.conseq) (insert P, auto simp: entail_def)
   thus ?thesis using i by (intro sound thread) auto
 qed
 
+(*
 text \<open>Refine via the elimination of verification conditions\<close>
 fun no_vc
   where 
@@ -407,6 +561,6 @@ proof -
   hence "R,G \<turnstile>\<^sub>s wp R G c Q {c} Q" using g wp_valid unfolding valid_def by blast
   hence "R,G \<turnstile>\<^sub>s P {c} Q" by (rule lrules.conseq) (insert P, auto simp: state_def entail_def)
   thus ?thesis using i no_vc_ref by (intro refine_sound thread) auto
-qed
+qed *)
 
 end
